MannaNess/AMannaNess.v
@@ -80,99 +80,73 @@ End manna_ness_hd_mod.
 
 Section rule_elimination.
 
-Variables R R' : rules.
+Variables R Rgt Rge : rules.
 
 Section mod.
 
-Variables E E' : rules.
+Variables E Egt Ege : rules.
+
+Lemma rule_elimination_mod : forall rp : Reduction_pair Sig,
+  compat (rp_succ    rp) Rgt ->
+  compat (rp_succ_eq rp) Rge -> 
+  compat (rp_succ    rp) Egt ->
+  compat (rp_succ_eq rp) Ege ->
+  WF (red_mod Ege Rge) ->
+  WF (red_mod (Egt ++ Ege) (Rgt ++ Rge)).
+
+Proof with auto.
+  intros. apply WF_incl with ((red Egt U red Ege)# @ (red Rgt U red Rge)).
+  comp. apply incl_rtc. trans (red Egt U red Ege)... apply red_union.
+  apply red_union.
+  apply wf_rel_mod...
+  apply WF_incl with ((red (Rge ++ Ege)# @ (red (Rgt ++ Egt)))).
+  comp. apply incl_rtc. apply red_union_inv.
+  apply red_union_inv.
+  apply manna_ness_mod with rp; apply compat_app...
+Qed.
+
+Lemma rule_elimination_hd_mod : forall wp : Weak_reduction_pair Sig,
+  compat (wp_succ_eq wp) E ->
+  compat (wp_succ_eq wp) Rge -> 
+  compat (wp_succ wp   ) Rgt ->
+  WF (hd_red_mod E Rge) -> 
+  WF (hd_red_mod E (Rgt ++ Rge)).
+
+Proof with auto.
+  intros. apply WF_incl with (red E # @ (hd_red Rgt U hd_red Rge)).
+  comp. apply hd_red_union. 
+  apply wf_rel_mod_simpl...
+  apply WF_incl with (hd_red_mod (Rge ++ E) Rgt).
+  comp. apply incl_rtc.
+  trans (red Rge U red E). union. apply hd_red_incl_red.
+  apply red_union_inv.
+  apply manna_ness_hd_mod with wp...
+  apply compat_app...
+Qed.
 
 Require Import Lexico.
 
-Lemma rule_elimination_mod : forall rp : Reduction_pair Sig,
-  compat (rp_succ_eq rp) E -> compat (rp_succ rp) E' ->
-  compat (rp_succ_eq rp) R -> compat (rp_succ rp) R' ->
-  WF (red_mod E R) -> WF (red_mod (E ++ E') (R ++ R')).
-
-Proof.
-intros. set (succ := rp_succ rp). set (succ_eq := rp_succ_eq rp).
-set (er := red_mod E R). set (F := E ++ E').
-(* h0 *)
-assert (h0 : er << succ_eq!). unfold er, succ_eq. incl_red.
-(* h1 *)
-assert (h1 : red F # << succ # @ red E #).
-trans ((red E U red E')#). apply incl_rtc. unfold F. apply red_union.
-trans (red_mod E E' # @ red E #). unfold red_mod. apply rtc_union.
-comp. apply incl_rtc. unfold succ. incl_red.
-(* h2 *)
-assert (h2 : red_mod F (R ++ R') << succ# @ er U succ!).
-trans (red_mod F R U red_mod F R'). apply red_mod_union. union.
-(* left *)
-unfold red_mod. trans ((succ # @ red E #) @ red R). comp. exact h1. assoc.
-(* right *)
-trans ((succ # @ red E #) @ red R'). unfold red_mod. comp. exact h1. assoc.
-trans (succ # @ succ). comp.
-trans (red_mod E R'). unfold succ. incl_red. apply rtc_step_incl_tc.
-(* h3 *)
-set (gt := succ! @ succ_eq#). assert (h3 : red_mod F (R ++ R') << er U gt).
-trans (succ# @ er U succ!). exact h2.
-trans ((er U succ! @ er) U succ!). union. apply rtc_comp.
-trans (er U (succ! @ er U succ!)). apply union_assoc. union.
-trans (succ! @ er%). apply union_fact2. unfold gt. comp.
-apply incl_rc_rtc. exact h0.
-(* h4 *)
-assert (h4 : succ_eq# @ succ! << succ!).
-apply comp_incl_tc. apply comp_rtc_incl. rptac.
-(* lexico *)
-eapply WF_incl with (S := lex' gt (er!)).
-trans (er U gt). exact h3. trans (er! U gt). union.
-apply tc_incl. trans (gt U er!). apply union_commut.
-apply lex'_intro. apply WF_lex'.
-(* WF gt *)
-unfold gt. apply WF_compat_inv. exact h4. apply WF_tc. WFtac.
-(* WF er! *)
-apply WF_tc. exact H3.
-(* er! trans *)
-apply tc_trans.
-(* compat *)
-apply comp_tc_incl. trans (succ_eq! @ gt). comp. exact h0.
-apply comp_tc_incl. unfold gt. assoc. comp. apply comp_incl_tc. rptac.
-Qed.
-
-Lemma weak_rule_elimination_mod : forall wp : Weak_reduction_pair Sig,
+Lemma rule_elimination_hd_mod_min : forall wp : Weak_reduction_pair Sig,
   compat (wp_succ_eq wp) E ->
-  compat (wp_succ_eq wp) R -> compat (wp_succ wp) R' ->
-  WF (hd_red_mod E R) -> WF (hd_red_mod E (R ++ R')).
-
-Proof.
-intros. set (succ := wp_succ wp). set (succ_eq := wp_succ_eq wp).
-set (er := hd_red_mod E R). set (er' := hd_red_mod E R').
-apply WF_incl with (S := lex' succ (er!)).
-trans (er U succ). trans (er U er'). unfold er, er'. apply hd_red_mod_union.
-union. unfold er', succ. incl_red.
-trans (succ U er). apply union_commut.
-trans (succ U er!). union. apply tc_incl.
-apply lex'_intro. apply WF_lex'. WFtac. apply WF_tc. exact H2. apply tc_trans.
-apply comp_tc_incl. trans (succ_eq! @ succ). comp. unfold er.
-trans (red_mod E R). apply hd_red_mod_incl_red_mod. incl_red.
-apply comp_tc_incl. rptac.
-Qed.
-
-Lemma weak_rule_elimination_mod_min : forall wp : Weak_reduction_pair Sig,
-  compat (wp_succ_eq wp) E ->
-  compat (wp_succ_eq wp) R -> compat (wp_succ wp) R' ->
-  WF (hd_red_mod_min E R) -> WF (hd_red_mod_min E (R ++ R')).
+  compat (wp_succ_eq wp) Rge -> 
+  compat (wp_succ wp   ) Rgt ->
+  WF (hd_red_mod_min E Rge) -> 
+  WF (hd_red_mod_min E (Rgt ++ Rge)).
 
 Proof.
   intros. set (succ := wp_succ wp). set (succ_eq := wp_succ_eq wp).
-  set (er := hd_red_mod_min E R). set (er' := hd_red_mod_min E R').
+  set (er := hd_red_mod_min E Rge). set (er' := hd_red_mod_min E Rgt).
   apply WF_incl with (S := lex' succ (er!)).
-  trans (er U succ). trans (er U er'). unfold er, er'. apply hd_red_mod_min_union.
+  trans (er U succ). trans (er U er').
+  trans (er' U er). unfold er, er'. apply hd_red_mod_min_union.
+  apply union_commut.
   union. unfold er', succ. incl_red.
   trans (succ U er). apply union_commut.
   trans (succ U er!). union. apply tc_incl.
-  apply lex'_intro. apply WF_lex'. WFtac. apply WF_tc. exact H2. apply tc_trans.
+  apply lex'_intro. apply WF_lex'. WFtac. apply WF_tc. 
+  exact H2. apply tc_trans.
   apply comp_tc_incl. trans (succ_eq! @ succ). comp. unfold er.
-  trans (red_mod E R). apply incl_trans with (hd_red_mod E R).
+  trans (red_mod E Rge). apply incl_trans with (hd_red_mod E Rge).
   apply hd_red_mod_min_incl. apply hd_red_mod_incl_red_mod. incl_red.
   apply comp_tc_incl. rptac.
 Qed.
@@ -180,36 +154,32 @@ Qed.
 End mod.
 
 Lemma rule_elimination : forall rp : Reduction_pair Sig,
-  compat (rp_succ_eq rp) R -> compat (rp_succ rp) R' ->
-  WF (red R) -> WF (red (R ++ R')).
+  compat (rp_succ_eq rp) Rge -> 
+  compat (rp_succ rp   ) Rgt ->
+  WF (red Rge) -> 
+  WF (red (Rgt ++ Rge)).
 
-Proof.
-intros. eapply WF_incl. apply red_incl_red_mod.
-change (WF (red_mod (nil++nil) (R++R'))). eapply rule_elimination_mod.
-unfold compat. simpl. intuition.
-unfold compat. simpl. intuition.
-apply H. apply H0.
-eapply WF_incl. apply red_mod_empty_incl_red. exact H1.
+Proof with auto.
+  intros. eapply WF_incl. apply red_incl_red_mod.
+  change (nil (A:=rule)) with (nil (A:=rule) ++ nil).
+  apply rule_elimination_mod with rp...
+  apply compat_empty. apply compat_empty.
+  apply WF_incl with (red Rge)... apply red_mod_empty_incl_red.
 Qed.
 
-Lemma weak_rule_elimination : forall wp : Weak_reduction_pair Sig,
-  compat (wp_succ_eq wp) R -> compat (wp_succ wp) R' ->
-  WF (hd_red R) -> WF (hd_red (R ++ R')).
+Lemma rule_elimination_hd_red : forall wp : Weak_reduction_pair Sig,
+  compat (wp_succ_eq wp) Rge -> 
+  compat (wp_succ wp   ) Rgt ->
+  WF (hd_red Rge) -> 
+  WF (hd_red (Rgt ++ Rge)).
 
-Proof.
-intros. eapply WF_incl. apply hd_red_incl_hd_red_mod.
-change (WF (hd_red_mod (nil++nil) (R++R'))). eapply weak_rule_elimination_mod.
-unfold compat. simpl. intuition.
-unfold compat. simpl. intuition.
-apply H0. eapply WF_incl. simpl. apply hd_red_mod_empty_incl_hd_red. exact H1.
+Proof with auto.
+  intros. eapply WF_incl. apply hd_red_incl_hd_red_mod.
+  apply rule_elimination_hd_mod with wp...
+  apply compat_empty.
+  apply WF_incl with (hd_red Rge)... apply hd_red_mod_empty_incl_hd_red.
 Qed.
 
 End rule_elimination.
-
-(*Lemma rule_filter : forall (rp : Reduction_pair Sig)
-  f (h : forall x y, f x y = true -> rp_succ rp x y) RR',
-  let f_rule a := match a with mkRule l r => f l r end in
-  let (R', R) := partition f_rule RR' in
-  compat (rp_succ_eq rp) R -> WF (red R) -> WF (red RR').*)
 
 End S.
