PolyInt/PolyChecker.v
@@ -1,0 +1,223 @@
+(**
+CoLoR, a Coq library on rewriting and termination.
+See the COPYRIGHTS and LICENSE files.
+
+- Adam Koprowski, 2009-03-24
+
+A termination solver using the polynomial interpretations method.
+*)
+
+Require Import Program.
+Require Import ListUtil.
+Require Import ListForall.
+Require Import LogicUtil.
+Require Import ZUtil.
+Require Import VecUtil.
+Require Import Problem.
+Require Import ATrs.
+Require Import SN.
+Require Import APolyInt.
+Require Import Polynom.
+Require Import RelUtil.
+Require Import MonotonePolynom.
+Require Import PositivePolynom.
+Require Import NaryFunction.
+Require Import MonAlgChecker.
+Require Import IntBasedChecker.
+Require Import Proof.
+Require Import ExcUtil.
+Require Import AWFMInterpretation.
+
+Set Implicit Arguments.
+
+Section PolySolver.
+
+Variable Sig : Signature.
+
+(***********************************************************************)
+(** checking polynomial interpretation and converting it to dependently
+    typed interpretation with constraints *)
+
+Program Definition check_mono (n : nat) (m : monomial) : Exc (Z * monom n) :=
+  match m with
+  | (coef, vars) =>
+      match eq_nat_dec n (List.length vars) with
+      | left _ => value (coef, vec_of_list vars)
+      | right _ => error
+      end
+  end.
+
+Definition check_poly (n : nat) (p : polynomial) : Exc (poly n) :=
+  map_exc (@check_mono n) p.
+
+Definition polyInt n := { p : poly n | pweak_monotone p }.
+
+Notation symPI := (symInt Sig polyInt).
+
+Program Definition symbol_poly_int (f : Sig) (p : polynomial) : Exc symPI :=
+  match check_poly (arity f) p with
+  | error => error
+  | value fi => 
+      match pweak_monotone_check fi with
+      | error => error
+      | value _ => value (buildSymInt Sig polyInt f fi)
+      end
+  end.
+
+Definition defaultPoly n : poly n :=
+  pconst n 1 ++ list_of_vec (Vbuild (fun i (ip : i < n) => (1%Z, mxi ip))).
+
+Lemma defaultPoly_mxi_1 n i (H : i < n) : In (1%Z, mxi H) (defaultPoly n).
+
+Proof.
+  intros. right. simpl.
+  apply list_of_vec_in.
+  rewrite <- (Vbuild_nth (fun i (ip : i < n) => (1%Z, mxi ip)) H).
+  apply Vnth_in.
+Qed.
+
+Lemma defaultPoly_wm n : pweak_monotone (defaultPoly n).
+
+Proof with simpl; auto with zarith.
+  intros. split... 
+  apply lforall_intro. intros.
+  ded (in_list_of_vec H).
+  ded (Vbuild_in (fun i ip => (1%Z, mxi ip)) x H0).
+  decomp_hyps. subst...
+Qed.
+
+Lemma defaultPoly_sm n : pstrong_monotone (defaultPoly n).
+
+Proof.
+  split. apply defaultPoly_wm.
+  intros. 
+  assert (HH : In (1%Z, mxi H) (defaultPoly n)).
+  apply defaultPoly_mxi_1.
+  set (w := coefPos_geC (defaultPoly n) (mxi H) 1 (defaultPoly_wm n) HH).
+  auto with zarith.
+Qed.
+
+Program Definition defaultInt n : polyInt n := defaultPoly n.
+
+Next Obligation.
+Proof.
+  set (w := defaultPoly_wm). simpl in w. apply w.
+Qed.
+
+Program Definition interpret n (fi : polyInt n) : naryFunction D n :=
+  @peval_D n fi _.
+
+Next Obligation.
+Proof.
+  destruct fi. hyp.
+Qed.
+
+(***********************************************************************)
+(** weak and strong monotonicity checking *)
+
+Program Definition poly_wm (fi : symPI) := True.
+Program Definition poly_sm (fi : symPI) := pstrong_monotone (projT2 fi).
+
+Lemma sm_imp_wm (fi : symPI) : poly_sm fi -> poly_wm fi.
+
+Proof.
+  firstorder.
+Qed.
+
+Program Definition check_wm (fi : symPI) : Exc (poly_wm fi) := 
+  value _.
+
+Next Obligation.
+Proof.
+  firstorder.
+Qed.
+
+Lemma wm_ok : forall fi, poly_wm fi -> Vmonotone (interpret (projT2 fi)) Dge.
+
+Proof.
+  intros. apply Vmonotone_transp. apply coef_pos_monotone_peval_Dle.
+Qed.
+
+Program Definition check_sm (fi : symPI) : Exc (poly_sm fi) :=
+  pstrong_monotone_check (projT2 fi).
+
+Lemma sm_ok : forall fi, poly_sm fi -> Vmonotone (interpret (projT2 fi)) Dgt.
+
+Proof.
+  intros. apply Vmonotone_transp. 
+  apply pmonotone_imp_monotone_peval_Dlt. hyp. 
+Qed.
+
+Let buildSymInt := buildSymInt Sig polyInt.
+Let defaultIntForSymbol := defaultIntForSymbol Sig polyInt defaultInt.
+
+Lemma default_sm : forall f, poly_sm (buildSymInt (defaultIntForSymbol f)).
+
+Proof.
+  intros. apply defaultPoly_sm.
+Qed.
+
+Definition wm_spec := Build_monSpec interpret poly_wm check_wm wm_ok.
+Definition sm_spec := Build_monSpec interpret poly_sm check_sm sm_ok.
+
+(***********************************************************************)
+(** rule compatibility with orders. *)
+
+Section Orders.
+
+Variable i : forall f : Sig, polyInt (arity f).
+
+Definition I := makeI Sig D0 polyInt interpret i.
+
+Let succ := IR I Dgt.
+Let succeq := IR I Dge.
+
+Program Definition check_succ (r : rule Sig) : Exc (succ (lhs r) (rhs r)) :=
+  match coef_pos_check (rulePoly_gt i r) with
+  | error => error
+  | value _ => value _
+  end.
+
+Next Obligation.
+Proof with try discriminate; auto.
+  destruct_call coef_pos_check...
+  apply pi_compat_rule...
+Qed.
+
+Program Definition check_succeq (r : rule Sig) : Exc (succeq (lhs r) (rhs r)) :=
+  match coef_pos_check (rulePoly_ge i r) with
+  | error => error
+  | value _ => value _
+  end.
+
+Next Obligation.
+Proof with try discriminate; auto.
+  destruct_call coef_pos_check...
+  apply pi_compat_rule_weak...
+Qed.
+
+End Orders.
+
+(***********************************************************************)
+(** solver for the technique of polynomial interpretations. *)
+
+Section solver.
+
+Variable int : rawTrsInt Sig polynomial.
+
+Definition succ_WF := WF_Dgt.
+
+Lemma succ_succeq_compat : absorb Dgt Dge.
+
+Proof.
+  intros p q pq. destruct pq as [r [pr rq]].
+  unfold Dgt, Dlt, transp. apply Zlt_le_trans with (val r); auto.
+Qed.
+
+Program Definition polySolver := monotoneAlgebraSolver succ_WF 
+  succ_succeq_compat defaultInt check_succ check_succeq wm_spec sm_spec 
+  sm_imp_wm default_sm int symbol_poly_int.
+
+End solver.
+
+End PolySolver.
