ProofChecker/EmptyChecker.v
@@ -1,0 +1,36 @@
+(**
+CoLoR, a Coq library on rewriting and termination.
+See the COPYRIGHTS and LICENSE files.
+
+- Adam Koprowski, 2009-03-24
+
+A termination solver that knows how to deal with empty problems.
+*)
+
+Require Import ListUtil.
+Require Import Problem.
+Require Import ATrs.
+Require Import SN.
+
+Set Implicit Arguments.
+
+Section EmptySolver.
+
+  Variable Sig : Signature.
+
+  Definition is_problem_empty (Pb : Problem Sig) :=
+    match Pb with
+    | FullTerm R => is_empty R
+    | RelTerm T R => is_empty R
+    | RelTopTerm T R => is_empty R
+    end.
+
+  Lemma empty_solver Pb : is_problem_empty Pb = true -> Prob_WF Pb.
+  Proof.
+    unfold Prob_WF; destruct Pb; simpl; intros; destruct R;
+      try solve [termination_trivial | discriminate].
+  Qed.
+
+End EmptySolver.
+
+Hint Resolve empty_solver : rainbow.
