ProofChecker/IntBasedChecker.v
@@ -1,0 +1,79 @@
+(**
+CoLoR, a Coq library on rewriting and termination.
+See the COPYRIGHTS and LICENSE files.
+
+- Adam Koprowski, 2009-03-25
+
+  A module with results for solvers using interpretations.
+*)
+
+Require Import Program.
+Require Import LogicUtil.
+Require Import ExcUtil.
+Require Import ListUtil.
+Require Import ListForall.
+Require Import ATrs.
+Require Import NaryFunction.
+Require Import AInterpretation.
+Require Import Proof.
+
+Set Implicit Arguments.
+
+Section IntBasedSolver.
+
+Variable Sig : Signature.
+
+Variable rawSymInt : Type.
+
+Definition rawTrsInt := trsInt Sig rawSymInt.
+
+Variable arSymInt : nat -> Set.
+
+Variable defaultInt : forall n, arSymInt n.
+
+Definition funInt (f : Sig) := arSymInt (arity f).
+Definition symInt := { f : Sig & funInt f }.
+
+Definition defaultIntForSymbol f := @defaultInt (@arity Sig f).
+
+Definition buildSymInt f fi : symInt := existT _ f fi.
+
+Variable checkInt : Sig -> rawSymInt -> Exc symInt.
+
+Fixpoint processInt (ri : rawTrsInt) : Exc (list symInt) :=
+  match ri with
+  | nil => value nil
+  | cons i is =>
+      match checkInt (fst i) (snd i) with
+      | error => error
+      | value fi => 
+          match processInt is with
+          | error => error
+          | value fis => value (fi :: fis)
+          end
+      end
+  end.
+
+Definition buildInt (i : list symInt) : forall f, funInt f :=
+  fun f => lookup_dep (el := f) (@eq_symb_dec Sig) defaultIntForSymbol i.
+
+Variable P : symInt -> Prop.
+Variable check_P : forall (i : symInt), Exc (P i).
+Variable default_P : forall f, P (buildSymInt (defaultIntForSymbol f)).
+
+Program Fixpoint checkProp (i : list symInt) : 
+  Exc (forall f, P (buildSymInt (buildInt i f))) :=
+
+  match lforall_exc P check_P i with
+  | error => error
+  | value _ => value _
+  end.
+
+Next Obligation.
+  apply (lookup_dep_prop (P := fun f fi => P (buildSymInt fi))); intros.
+  destruct_call lforall_exc; try discr.
+  ded (lforall_in l H). decomp_hyp H0. destruct x. hyp.
+  apply default_P.
+Qed.
+
+End IntBasedSolver.
