ProofChecker/Problem.v
@@ -1,0 +1,39 @@
+(**
+CoLoR, a Coq library on rewriting and termination.
+See the COPYRIGHTS and LICENSE files.
+
+- Adam Koprowski, 2009-03-24
+
+A specification of a termination problem.
+*)
+
+Require Import List.
+Require Import Relations.
+Require Import ATrs.
+Require Import SN.
+
+Set Implicit Arguments.
+
+Section TerminationProblem.
+
+  Variable Sig : Signature.
+
+  Notation term := (term Sig).
+  Notation rule := (rule Sig).
+  Notation trs := (list rule).
+
+  Inductive Problem : Type :=
+  | FullTerm (R : trs)
+  | RelTerm (T R : trs)
+  | RelTopTerm (T R : trs).
+
+  Definition prob_red (P : Problem) : relation term :=
+    match P with
+    | FullTerm R => red R
+    | RelTerm T R => red_mod T R
+    | RelTopTerm T R => hd_red_mod T R
+    end.
+
+  Definition Prob_WF (P : Problem) := WF (prob_red P).
+
+End TerminationProblem.
