ProofChecker/ProofChecker.v
@@ -1,0 +1,59 @@
+(**
+CoLoR, a Coq library on rewriting and termination.
+See the COPYRIGHTS and LICENSE files.
+
+- Adam Koprowski, 2009-03-24
+
+A machinery to check termination proofs.
+*)
+
+Require Import Relations.
+Require Import List.
+Require Import SN.
+Require Import ATrs.
+Require Import ARelation.
+Require Import Problem.
+Require Import Proof.
+Require Import EmptyChecker.
+Require PolyChecker.
+
+Set Implicit Arguments.
+
+Section ProofChecker.
+
+Variable Sig : Signature.
+
+Inductive TerminationAnalysisResult (P : Problem Sig) :=
+| TerminationEstablished (Prf : Prob_WF P)
+| Error.
+
+Implicit Arguments TerminationEstablished [P].
+Implicit Arguments Error [P].
+
+Program Fixpoint check_proof (Pb : Problem Sig) (Prf : TerminationProof Sig) 
+  {struct Prf} : TerminationAnalysisResult Pb :=
+
+  match Prf with
+  | TP_PolyInt PI Prf' =>
+      match PolyChecker.polySolver PI Pb with
+      | error => Error
+      | value Pb' => 
+          match check_proof Pb' Prf' with
+          | Error => Error
+          | TerminationEstablished _ => TerminationEstablished _
+          end
+      end
+
+  | TP_ProblemEmpty => 
+      match EmptyChecker.is_problem_empty Pb with
+      | true => TerminationEstablished _
+      | _ => Error
+      end
+  end.
+
+Next Obligation.
+Proof.
+  auto with rainbow.
+Qed.
+
+End ProofChecker.
