Util/Option/ExcUtil.v
@@ -1,0 +1,115 @@
+(**
+CoLoR, a Coq library on rewriting and termination.
+See the COPYRIGHTS and LICENSE files.
+
+- Adam Koprowski, 2009-03-27
+
+  Utility results about the option/exception type.
+*)
+
+Require Import Bool.
+Require Import ListForall.
+Require Import ListUtil.
+Require Import Program.
+
+Set Implicit Arguments.
+
+Section ExcUtil.
+
+Variable A : Type.
+Variable P : A -> Prop.
+Variable f : forall a : A, Exc (P a).
+
+Definition exc_to_bool (P : Prop) (e : Exc P) :=
+  match e with
+  | value _ => true
+  | error => false
+  end.
+
+Definition pred_exc_to_bool x := exc_to_bool (f x).
+
+Program Definition lforall_exc (l : list A) : 
+  Exc (lforall (fun x : A => exists p, f x = value p) l) :=
+  match forallb pred_exc_to_bool l with
+  | true => value _
+  | false => error
+  end.
+
+Next Obligation.
+Proof with auto.
+  apply forallb_imp_lforall with (fun x => exc_to_bool (f x))...
+  intros. destruct (f x). exists p... discriminate.
+Qed.
+
+Program Definition partition_exc (l : list A) :
+  { ll : list A * list A |
+      let (l1, l2) := ll in
+        lforall P l1 /\
+        (lforall (fun x => f x = error) l2) /\
+        (forall x, In x l -> In x l1 \/ In x l2)
+        
+  } :=
+  partition pred_exc_to_bool l.
+
+Next Obligation.
+Proof with auto.
+  assert (left := fun x => partition_left pred_exc_to_bool x l).
+  assert (right := fun x => partition_right pred_exc_to_bool x l).
+  assert (complete := fun x => partition_complete pred_exc_to_bool x l).
+  destruct (partition pred_exc_to_bool l).
+  unfold pred_exc_to_bool in *.
+  repeat split...
+  apply lforall_intro. intros x xl.
+  assert (ll := left x xl). destruct (f x); try discriminate...
+  apply lforall_intro. intros x xl.
+  assert (rr := right x xl). destruct (f x); try discriminate...
+Qed.
+
+End ExcUtil.
+
+Section MapExc.
+
+Variable A B : Type.
+Variable f : A -> Exc B.
+
+Program Fixpoint map_exc (l : list A) : Exc (list B) :=
+  match l with
+  | [] => value []
+  | cons x xs => 
+      match f x with
+      | error => error
+      | value v =>
+          match map_exc xs with
+          | error => error
+          | value vs => value (v :: vs)
+          end
+      end
+  end.
+
+End MapExc.
+
+(* Anomaly: *)
+(*
+Section Error.
+
+Variable A B : Type.
+Variable f : A -> B.
+
+Program Fixpoint map_exc (l : list A) : Exc (list B) :=
+  match l with
+  | [] => value []
+  | cons x xs => 
+      match f x with
+      | error => error
+      | value v =>
+          match map_exc xs with
+          | error => error
+          | value vs => value (v :: vs)
+          end
+      end
+  end.
+
+End Error.
+*)
+
+Implicit Arguments exc_to_bool [P].
